theories/ftlr/JmpCap.v
@@ -50,9 +50,6 @@ Section fundamental.
       (* apply IH *)
       iApply ("IH" $! _ _ _ _ g _ _ a with "[] [] [Hmap] [$Hr] [$Hsts] [$Hown]"); eauto.
       { iPureIntro; apply Hsome. }
-      destruct p
-      ; iFrame
-      ; apply isCorrectPC_nonSentry in HcorrectPC; by cbn in HcorrectPC.
     - specialize Hsome with rsrc as Hrsrc; destruct Hrsrc as [wsrc Hsomesrc].
       iExtract "Hmap" rsrc as "Hrsrc".
       iApply (wp_jmpcap_success with "[$HPC $Ha $Hrsrc]"); eauto.
@@ -61,7 +58,7 @@ Section fundamental.
       (* reconstruct regions *)
       iInsert "Hmap" rsrc;
       rewrite -delete_insert_ne; auto.
-      destruct (updatePcPerm wsrc) eqn:Heq ; [ | destruct sb | ]; cycle 1.
+      destruct (updatePcPerm wsrc) eqn:Heq ; [ | destruct sb | | ]; cycle 1.
       { destruct (executeAllowed p0) eqn:Hpft; cycle 1.
         { iNext; iIntros "_".
           iApply (wp_bind (fill [SeqCtx])).
@@ -73,14 +70,18 @@ Section fundamental.
         iInsert "Hmap" PC.
         rewrite (insert_id regs rsrc); auto.
         iDestruct ("Hreg" $! rsrc _ HrPC Hsomesrc) as "Hwsrc".
-        destruct wsrc; simpl in Heq; try congruence.
-        destruct sb as [p1 g1 b1 e1 a1|?]; try congruence.
-        destruct p1 as [rx pw dl dro | rx pw dl dro] ; cycle 1; simplify_eq.
-        + (* case p1 = E *)
+        destruct wsrc; simpl in Heq; try congruence; simplify_eq.
+        - (* case cap *)
+          iEval (rewrite fixpoint_interp1_eq) in "Hinv_interp".
+          iNext; iIntros "_".
+          iDestruct (region_close with "[$Hstate $Hr Hw $Ha $HmonoV]") as "Hr"; eauto.
+          { destruct ρ;auto;[|ospecialize (Hnotfrozen _)];contradiction. }
+          iApply ("IH" with "[] [] [$Hmap] [$Hr] [$Hsts] [$Hown]"); eauto.
+        - (* case sentry *)
           iEval (rewrite fixpoint_interp1_eq) in "Hwsrc".
           simpl; rewrite /enter_cond.
           iDestruct "Hwsrc" as "#H".
-          destruct ( decide (WCap (E rx pw dl dro) g0 b0 e0 a0 = switcher_ret_entry_point) ) as [? |?].
+          destruct ( decide (WSentry p0 g0 b0 e0 a0 = switcher_ret_entry_point) ) as [? |?].
           * rewrite (decide_True ( P:= (_ = switcher_ret_entry_point))); last done.
             rewrite switcher_ret_correct in e1; simplify_eq.
             iAssert (future_world Local W W) as "Hfuture".
@@ -100,12 +101,6 @@ Section fundamental.
             { destruct ρ;auto;[|ospecialize (Hnotfrozen _)];contradiction. }
             iDestruct ("H" with "[$Hmap $Hr $Hsts $Hown]") as "HA"; eauto.
             iFrame "#%".
-        + (* case p1 ≠ E *)
-          iEval (rewrite fixpoint_interp1_eq) in "Hinv_interp".
-          iNext; iIntros "_".
-          iDestruct (region_close with "[$Hstate $Hr Hw $Ha $HmonoV]") as "Hr"; eauto.
-          { destruct ρ;auto;[|ospecialize (Hnotfrozen _)];contradiction. }
-          iApply ("IH" with "[] [] [$Hmap] [$Hr] [$Hsts] [$Hown]"); eauto.
       }
 
       (* Non-capability cases *)
